theory/x64EncodeProof.thy
@@ -3,12 +3,12 @@ imports
   Main
   rBPFCommType
   x64Assembler x64Disassembler
-(*  x64_encode_movl_rr_1 x64_encode_movl_rr_3
-  x64_encode_movl_rr_4 x64_encode_movl_rr_5 x64_encode_movl_rr_6
+(*  x64_encode_movl_rr_1 x64_encode_movl_rr_3  x64_encode_movl_rr_4 x64_encode_movl_rr_5 x64_encode_movl_rr_6
   x64_encode_movq_rr_1
   x64_encode_mov_rm_1 x64_encode_mov_rm_2 x64_encode_mov_rm_3 x64_encode_mov_rm_4
-  x64_encode_cmovl_1 x64_encode_cmovl_2 x64_encode_cmovl_3*)
-  x64_encode_cmovq_1
+  x64_encode_cmovl_1 x64_encode_cmovl_2 x64_encode_cmovl_3
+  x64_encode_cmovq_1*)
+  x64_encode_cqo_1
 begin
 
 declare if_split_asm [split]
@@ -32,7 +32,7 @@ lemma x64_decode_encode_consistency:
   apply (cases ins; simp_all)
 
 
-                      prefer 10
+                      prefer 15
 
 
 
@@ -196,6 +196,57 @@ Proof done
       done
     done
           
+  subgoal for dst src
+  \<comment> \<open> Pxchgq_rr 10\<close> 
+    apply (unfold construct_rex_to_u8_def construct_modsib_to_u8_def)
+    apply (unfold x64_decode_def Let_def, auto simp add: split: option.splits)
+    apply (cases l_bin, simp_all)
+    subgoal for l_bin1
+      apply (cases l_bin1, simp_all)
+      subgoal for l_bin2
+        apply (cases l_bin2, simp_all)
+        subgoal for t l_bin3
+          subgoal
+            using encode_movq_rr_1 by blast
+          done
+        done
+      done
+    done
+
+  subgoal for dst src
+  \<comment> \<open> Pmovsq_rr 12\<close> 
+    apply (unfold construct_rex_to_u8_def construct_modsib_to_u8_def)
+    apply (unfold x64_decode_def Let_def, auto simp add: split: option.splits)
+    apply (cases l_bin, simp_all)
+    subgoal for l_bin1
+      apply (cases l_bin1, simp_all)
+      subgoal for l_bin2
+        apply (cases l_bin2, simp_all)
+        subgoal for t l_bin3
+          subgoal
+            using encode_movq_rr_1 by blast
+          done
+        done
+      done
+    done
+
+  subgoal
+  \<comment> \<open> Pcdq 13\<close> 
+    apply (unfold x64_decode_def Let_def, auto simp add: split: option.splits)
+    apply (cases l_bin, simp_all)
+    done
+
+  subgoal
+  \<comment> \<open> Pcqo 14\<close> 
+    apply (unfold x64_decode_def Let_def,auto simp add: split: option.splits)
+    apply (cases l_bin, simp_all)
+    subgoal for l_bin1
+      apply (cases l_bin1, simp_all)
+      subgoal for t l_bin2
+        using x64_encode_cqo_1 by blast
+      done
+    done
+  done
 
 
 *)
