theory/x64_encode_cqo_1.thy
@@ -1,0 +1,68 @@
+theory x64_encode_cqo_1
+imports
+  Main
+  rBPFCommType
+  x64Syntax BitsOpMore
+begin
+
+
+lemma x64_encode_cqo_1: "    and 15 ((v::u8) >> 4) = 4 \<Longrightarrow> 
+    bit v 3 \<Longrightarrow> \<not> bit v 2 \<Longrightarrow> \<not> bit v (Suc 0) \<Longrightarrow> and 1 v = 0 \<Longrightarrow>  v = 72"
+  apply (rule bit_eqI)
+  apply (auto simp add: bit_simps)
+
+  subgoal for n
+    subgoal
+      apply (cases n, simp_all)
+      subgoal
+        by (simp add: bit_0 even_iff_mod_2_eq_zero one_and_eq)
+      subgoal for n1 apply (cases n1, simp_all)
+        subgoal for n2 apply (cases n2, simp_all)
+          subgoal
+            by (metis numeral_2_eq_2)
+          subgoal for n3 apply (cases n3, simp_all)
+            subgoal for n4 apply (cases n4, simp_all)
+              subgoal
+                by (metis add_2_eq_Suc' bit_1_0 bit_and_iff bit_numeral_Bit1_0 bit_word_iff_drop_bit_and not_bit_numeral_Bit0_0 numeral_2_eq_2 numeral_Bit0)
+              subgoal for n5 apply (cases n5, simp_all)
+                subgoal for n6 apply (cases n6, simp_all)
+                  done
+                done
+              done
+            done
+          done
+        done
+      done
+    done
+
+  subgoal for n
+    subgoal
+      apply (cases n, simp_all)
+      subgoal for n1 apply (cases n1, simp_all)
+        subgoal for n2 apply (cases n2, simp_all)
+          subgoal for n3 apply (cases n3, simp_all)
+            subgoal
+              using numeral_3_eq_3 by argo 
+            subgoal for n4 apply (cases n4, simp_all)
+              subgoal for n5 apply (cases n5, simp_all)
+                subgoal for n6 apply (cases n6, simp_all)
+                  done
+                done
+              done
+            done
+          done
+        done
+      done
+    done
+  done
+
+
+
+
+
+
+
+
+
+
+end
